Prove all equalities in coq

helpers/teq_coq/teq.v
@@ -41,6 +41,7 @@ Fixpoint shift (i : nat) (t : Term) : Term :=
   end.
 Definition Shift := shift 0.
 Definition Shift1 := shift 1.
+
 Fixpoint Shift' (n : nat) (t : Term) : Term :=
   match n with
   | 0 => t
@@ -70,4 +71,300 @@ Fixpoint sub (i : nat) (V t : Term) :=
   | trefl A a => trefl (sub i V A) (sub i V a)
   | teq A a b => teq (sub i V A) (sub i V a) (sub i V b)
   end.
+Definition apply1 (t1 t2 : Term) := sub 0 t2 t1.
 
+Ltac rewrite_all' :=
+  match goal with
+  | H : _ |- _ => rewrite H by auto; rewrite_all'
+  | _ => idtac
+  end.
+Ltac fold_Shift' :=
+  match goal with
+  | |- context[Shift (Shift' ?n ?u)]
+      => change (Shift (Shift' n u)) with (Shift' (S n) u); fold_Shift'
+  | _ => idtac
+  end.
+
+Hint Resolve le_n_S : core.
+Hint Extern 0 => rewrite_all' : core.
+
+Lemma ordered_integers (i j n : nat) :
+  j <= i ->
+  n <= j \/ (j < n /\ n <= i) \/ i < n.
+Proof.
+  intro Hij.
+  induction n.
+  - destruct j; auto. left. apply le_0_n.
+  - destruct Hij; destruct IHn as [ Hnj | [ [ Hjn Hni ] | Hin ] ]; auto.
+    + destruct Hnj; auto.
+    + destruct Hnj; auto.
+    + destruct Hni; auto.
+      right. left. split; auto.
+Qed.
+
+Lemma dbshift_spec1 (i j : nat) :
+  i <= j -> dbshift i j = S j.
+Proof.
+  generalize dependent i.
+  induction j; intros i H; destruct i; auto.
+  - inversion H.
+  - simpl. f_equal. apply IHj.
+    apply le_S_n. assumption.
+Qed.
+
+Lemma dbshift_spec2 (i j : nat) :
+  j < i -> dbshift i j = j.
+Proof.
+  generalize dependent i.
+  induction j; intros i H; destruct i; auto.
+  - inversion H.
+  - inversion H.
+  - simpl. f_equal. apply IHj.
+    unfold lt in *. apply le_S_n. assumption.
+Qed.
+
+Lemma dbselect_spec_lt (i j : nat) (eqT gtT ltT : Term) :
+  i < j -> dbselect i j eqT gtT ltT = ltT.
+Proof.
+  generalize dependent i.
+  induction j; intros i H; destruct i; simpl; auto.
+  - inversion H.
+  - inversion H.
+  - apply IHj. unfold lt in *. apply le_S_n. assumption.
+Qed.
+
+Lemma dbselect_spec_eq (i j : nat) (eqT gtT ltT : Term) :
+  i = j -> dbselect i j eqT gtT ltT = eqT.
+Proof.
+  intro H. subst. induction j; auto.
+Qed.
+
+Lemma dbselect_spec_gt (i j : nat) (eqT gtT ltT : Term) :
+  i > j -> dbselect i j eqT gtT ltT = gtT.
+Proof.
+  unfold gt. unfold lt. generalize dependent i.
+  induction j; intros i H; destruct i; simpl; auto.
+  - inversion H.
+  - inversion H.
+  - apply IHj. apply le_S_n. assumption.
+Qed.
+
+Lemma teq_shift_shift (i j : nat) (u : Term) :
+  i <= j -> shift i (shift j u) = shift (S j) (shift i u).
+Proof.
+  generalize dependent j. generalize dependent i.
+  induction u; intros i j H; simpl; auto.
+  f_equal. generalize dependent j. generalize dependent i.
+  induction n; intros i j Hij; simpl.
+  { destruct i; simpl; try reflexivity.
+    destruct Hij; simpl; reflexivity.
+  }
+  { destruct i; destruct j; simpl; auto.
+    - inversion Hij.
+    - f_equal. apply IHn. apply le_S_n. assumption.
+  }
+Qed.
+Lemma teq_shift_shift0 (i : nat) (u : Term) :
+  Shift (shift i u) = shift (S i) (Shift u).
+Proof.
+  apply teq_shift_shift. apply le_0_n.
+Qed.
+
+Lemma teq_shift_dbselect (n i j : nat) (eqT gtT ltT : Term) :
+  shift n (dbselect i j eqT gtT ltT) = dbselect i j (shift n eqT) (shift n gtT) (shift n ltT).
+Proof.
+  generalize dependent j.
+  induction i; intro j; destruct j; auto.
+  simpl. apply IHi.
+Qed.
+Lemma teq_shift_dbselect0 (i j : nat) (eqT gtT ltT : Term) :
+  Shift (dbselect i j eqT gtT ltT) = dbselect i j (Shift eqT) (Shift gtT) (Shift ltT).
+Proof.
+  unfold Shift. apply teq_shift_dbselect.
+Qed.
+Lemma teq_dbselect_Sn (i n : nat) (eqT gtT : Term) :
+  dbselect i n eqT gtT (var n) = dbselect i n eqT gtT (var (S (dbprev n))).
+Proof.
+  induction i; induction n; reflexivity.
+Qed.
+
+Ltac raise_dbselect :=
+  match goal with
+  | |- context[shift ?n (dbselect ?i ?j ?e ?g ?l)]
+  (*| |- context[dbselect ?i ?j (shift ?n ?e) (shift ?n ?g) (shift ?n ?l)] *)
+      => rewrite -> (teq_shift_dbselect n i j e g l); raise_dbselect
+  | |- context[Shift (dbselect ?i ?j ?e ?g ?l)]
+      => rewrite -> (teq_shift_dbselect0 i j e g l); raise_dbselect
+  | _ => idtac
+  end.
+Ltac pop_shift :=
+  match goal with
+  | |- context[dbselect ?i ?j (shift ?n ?e) (shift ?n ?g) (shift ?n ?l)]
+      => rewrite <- (teq_shift_dbselect n i j e g l); pop_shift
+  | |- context[dbselect ?i ?n ?eqT ?gtT (var ?n)]
+      => rewrite -> (teq_dbselect_Sn i n eqT gtT); pop_shift
+  | |- context[var (S ?n)]
+      => change (var (S n)) with (Shift (var n)); pop_shift
+  | |- context[shift (S ?n) (Shift ?u)]
+      => rewrite <- (teq_shift_shift0 n u); pop_shift
+  | |- context[dbselect ?i ?j (Shift ?e) (Shift ?g) (Shift ?l)]
+      => rewrite <- (teq_shift_dbselect0 i j e g l); pop_shift
+  | _ => idtac
+  end.
+Ltac push_shift :=
+  match goal with
+  | |- context[Shift (dbselect ?i ?j ?eqT ?gtT ?ltT)]
+      => rewrite -> (teq_shift_dbselect0 i j eqT gtT ltT); push_shift
+  | |- context[Shift (shift ?n ?u)]
+      => rewrite -> (teq_shift_shift0 n u); push_shift
+  | |- context[Shift (var ?n)]
+      => change (Shift (var n)) with (var (S n)); push_shift
+  | |- context[dbselect ?i ?n ?eqT ?gtT (var (S (dbprev ?n)))]
+      => rewrite <- (teq_dbselect_Sn i n eqT gtT); push_shift
+  | _ => idtac
+  end.
+
+Lemma teq_subst_shift (i j : nat) (u t : Term) :
+  j <= i ->
+  sub (S i) (shift j (Shift' j u)) (shift j t) = shift j (sub i (Shift' j u) t).
+Proof.
+  generalize dependent u.
+  generalize dependent j. generalize dependent i.
+  induction t; intros i j u Hij; simpl; push_shift; fold_Shift'; auto.
+  generalize dependent j. generalize dependent i.
+  induction n; intros i j Hij; simpl.
+  - destruct i; destruct j; simpl; try reflexivity. inversion Hij.
+  - destruct i; destruct j; simpl.
+    + reflexivity.
+    + inversion Hij.
+    + raise_dbselect. reflexivity.
+    + remember (dbshift j n) as djn. pose (IH := (IHn i j)). rewrite <- Heqdjn in IH.
+      destruct djn; pop_shift; f_equal; push_shift; apply IH; apply le_S_n; assumption.
+Qed.
+
+Lemma LP_teq_subst_shift (i : nat) (u t : Term) :
+  sub (S i) (Shift u) (Shift t) = Shift (sub i u t).
+Proof.
+  unfold Shift. change u with (Shift' 0 u).
+  apply (teq_subst_shift i 0 u t). apply le_0_n.
+Qed.
+Lemma LP_teq_subst_shift1 (i : nat) (u t : Term) :
+  sub (S (S i)) (Shift (Shift u)) (Shift1 t)
+  = Shift1 (sub (S i) (Shift u) t).
+Proof.
+  unfold Shift. rewrite teq_shift_shift0. unfold Shift.
+  change (shift 0 u) with (Shift' 1 u). unfold Shift1.
+  apply teq_subst_shift. apply le_n_S. apply le_0_n.
+Qed.
+Lemma LP_teq_select_shift (i id : nat) (V : Term) :
+  dbselect (S i) (S id) (Shift V) (var (S id)) (var id)
+  = Shift (dbselect i id V (var id) (var (dbprev id))).
+Proof.
+  simpl. pop_shift. reflexivity.
+Qed.
+
+Ltac pop_shift ::=
+  match goal with
+  | |- context[dbselect ?i ?j (shift ?n ?e) (shift ?n ?g) (shift ?n ?l)]
+      => rewrite <- (teq_shift_dbselect n i j e g l); pop_shift
+  | |- context[dbselect ?i ?n ?eqT ?gtT (var ?n)]
+      => rewrite -> (teq_dbselect_Sn i n eqT gtT); pop_shift
+  | |- context[var (S ?n)]
+      => change (var (S n)) with (Shift (var n)); pop_shift
+  | |- context[shift (S ?n) (Shift ?u)]
+      => rewrite <- (teq_shift_shift0 n u); pop_shift
+  | |- context[dbselect ?i ?j (Shift ?e) (Shift ?g) (Shift ?l)]
+      => rewrite <- (teq_shift_dbselect0 i j e g l); pop_shift
+  | |- context[sub (S ?i) (Shift ?u) (Shift ?t)]
+      => rewrite -> (LP_teq_subst_shift i u t); pop_shift
+  | _ => idtac
+  end.
+Ltac push_shift ::=
+  match goal with
+  | |- context[Shift (sub ?i ?u ?t)]
+      => rewrite <- (LP_teq_subst_shift i u t); push_shift
+  | |- context[Shift (dbselect ?i ?j ?eqT ?gtT ?ltT)]
+      => rewrite -> (teq_shift_dbselect0 i j eqT gtT ltT); push_shift
+  | |- context[Shift (shift ?n ?u)]
+      => rewrite -> (teq_shift_shift0 n u); push_shift
+  | |- context[Shift (var ?n)]
+      => change (Shift (var n)) with (var (S n)); push_shift
+  | |- context[dbselect ?i ?n ?eqT ?gtT (var (S (dbprev ?n)))]
+      => rewrite <- (teq_dbselect_Sn i n eqT gtT); push_shift
+  | _ => idtac
+  end.
+
+Lemma teq_subst_dbselect (i j k : nat) (u eqT gtT ltT : Term) :
+  sub k u (dbselect i j eqT gtT ltT) = dbselect i j (sub k u eqT) (sub k u gtT) (sub k u ltT).
+Proof.
+  generalize dependent j.
+  induction i; intro j; destruct j; simpl; try reflexivity.
+  apply IHi.
+Qed.
+
+Lemma dbshift_spec (i n : nat) :
+  (dbshift i n = n /\ dbshift i n < i)
+  \/ (dbshift i n = S n /\ dbshift i n > i).
+Proof.
+  generalize dependent n. induction i; intro n; simpl.
+  - right. split; try reflexivity. unfold gt. unfold lt. apply le_n_S. apply le_0_n.
+  - destruct n; simpl.
+    + left. split; try reflexivity. unfold lt. apply le_n_S. apply le_0_n.
+    + destruct (IHi n) as [ [ Heq H ] | [ Heq H ] ]; [ left | right ];
+        rewrite Heq in *; split; try reflexivity;
+        unfold gt in *; unfold lt in *; auto using le_n_S.
+Qed.
+
+Lemma teq_shift_cancel_subst (i : nat) (u t : Term) :
+  sub i u (shift i t) = t.
+Proof.
+  generalize dependent i. generalize dependent u.
+  induction t; simpl; try (intros u i; rewrite_all'; reflexivity).
+  induction n; intros u i; destruct i; simpl; try reflexivity.
+  pop_shift. destruct (dbshift_spec i n) as [ [ Heq H ] | [ Heq H ] ].
+  - rewrite dbselect_spec_gt by (unfold gt; assumption).
+    rewrite Heq. reflexivity.
+  - push_shift. rewrite dbselect_spec_lt by (unfold gt in H; assumption).
+    rewrite Heq. reflexivity.
+Qed.
+
+Lemma teq_subst_subst (i j : nat) (u t1 t2 : Term) :
+  j <= i ->
+  sub i (Shift' i u) (sub j (Shift' j t1) t2)
+  = sub j (sub i (Shift' i u) (Shift' j t1)) (sub (S i) (Shift' (S i) u) t2).
+Proof.
+  generalize dependent t1. generalize dependent u.
+  generalize dependent j. generalize dependent i.
+  induction t2;
+    try (intros i j u t1 Hij; simpl; fold_Shift';
+         rewrite_all'; simpl; push_shift; fold_Shift'; reflexivity).
+  induction n; intros i j u t1 Hij;
+    destruct i; destruct j; simpl; try reflexivity.
+  - inversion Hij.
+  - destruct n; simpl; try reflexivity. unfold Shift.
+    symmetry. change (sub 0 u t1) with (Shift' 0 (sub 0 u t1)).
+    apply teq_shift_cancel_subst.
+  - inversion Hij.
+  - destruct n; simpl; try reflexivity. simpl in IHn.
+    pop_shift. unfold Shift.
+    change (sub (S i) (shift 0 (Shift' i u)) t1)
+      with (Shift' 0 (sub (S i) (shift 0 (Shift' i u)) t1)).
+    rewrite teq_shift_cancel_subst. reflexivity.
+  - destruct n; simpl; pop_shift; f_equal; simpl in IHn;
+      push_shift; apply IHn; apply le_S_n; assumption.
+Qed.
+
+Lemma LP_teq_subst_apply (i : nat) (u t1 t2 : Term) :
+  sub i (Shift' i u) (apply1 t2 t1)
+  = apply1 (sub (S i) (Shift' (S i) u) t2) (sub i (Shift' i u) t1).
+Proof.
+  unfold apply1. change t1 with (Shift' 0 t1).
+  apply teq_subst_subst. apply le_0_n.
+Qed.
+
+Lemma LP_teq_shift_cancel_subst (i : nat) (u t : Term) :
+  sub i u (shift (S i) (shift i t)) = shift i t.
+Proof.
+  rewrite <- teq_shift_shift by constructor.
+  apply teq_shift_cancel_subst.
+Qed.
